

Multi-class classification with Softmax function

Lê Anh Cường

Outline

- Repeat logistic function
- Softmax function
- Derivative of the softmax function

Logistic function

$$\sigma(\mathbf{z}) = \frac{\mathbf{1}}{\mathbf{1} + e^{-\mathbf{z}}}$$

$$h_{\theta}(x) = P(y = 1|x; \theta) = \frac{\mathbf{1}}{\mathbf{1} + e^{-\theta^T x}}$$

$$P(y = 0|x; \theta) = 1 - P(y = 1|x; \theta) = \frac{e^{-\theta^T x}}{\mathbf{1} + e^{-\theta^T x}}$$

Softmax function

The [logistic output function](#) described in the previous section can only be used for the classification between two target classes $t = 1$ and $t = 0$. This logistic function can be generalized to output a multiclass categorical probability distribution by the [softmax function](#). This softmax function ς takes as input a C -dimensional vector \mathbf{z} and outputs a C -dimensional vector \mathbf{y} of real values between 0 and 1. This function is a normalized exponential and is defined as:

$$y_c = \varsigma(\mathbf{z})_c = \frac{e^{z_c}}{\sum_{d=1}^C e^{z_d}} \quad \text{for } c = 1 \dots C$$

Softmax function

The denominator $\sum_{d=1}^C e^{z_d}$ acts as a regularizer to make sure that $\sum_{c=1}^C y_c = 1$. As the output layer of a neural network, the softmax function can be represented graphically as a layer with C neurons.

We can write the probabilities that the class is $t = c$ for $c = 1 \dots C$ given input \mathbf{z} as:

$$\begin{bmatrix} P(t = 1|\mathbf{z}) \\ \vdots \\ P(t = C|\mathbf{z}) \end{bmatrix} = \begin{bmatrix} \varsigma(\mathbf{z})_1 \\ \vdots \\ \varsigma(\mathbf{z})_C \end{bmatrix} = \frac{1}{\sum_{d=1}^C e^{z_d}} \begin{bmatrix} e^{z_1} \\ \vdots \\ e^{z_C} \end{bmatrix}$$

Where $P(t = c|\mathbf{z})$ is thus the probability that that the class is c given the input \mathbf{z} .

Derivative of the softmax function

To use the softmax function in neural networks, we need to compute its derivative. If we define $\Sigma_C = \sum_{d=1}^C e^{z_d}$ for $c = 1 \cdots C$ so that $y_c = e^{z_c} / \Sigma_C$, then this derivative $\partial y_i / \partial z_j$ of the output \mathbf{y} of the softmax function with respect to its input \mathbf{z} can be calculated as:

$$\begin{aligned} \text{if } i = j : \frac{\partial y_i}{\partial z_i} &= \frac{\partial \frac{e^{z_i}}{\Sigma_C}}{\partial z_i} = \frac{e^{z_i} \Sigma_C - e^{z_i} e^{z_i}}{\Sigma_C^2} = \frac{e^{z_i}}{\Sigma_C} \frac{\Sigma_C - e^{z_i}}{\Sigma_C} = \frac{e^{z_i}}{\Sigma_C} \left(1 - \frac{e^{z_i}}{\Sigma_C}\right) = y_i(1 - y_i) \\ \text{if } i \neq j : \frac{\partial y_i}{\partial z_j} &= \frac{\partial \frac{e^{z_i}}{\Sigma_C}}{\partial z_j} = \frac{0 - e^{z_i} e^{z_j}}{\Sigma_C^2} = -\frac{e^{z_i}}{\Sigma_C} \frac{e^{z_j}}{\Sigma_C} = -y_i y_j \end{aligned}$$

Note that if $i = j$ this derivative is similar to the derivative of the logistic function.

Cross-entropy loss function for the softmax function

The likelihood $\mathcal{L}(\theta|\mathbf{t}, \mathbf{z})$ can be rewritten as the **joint probability** of generating \mathbf{t} and \mathbf{z} given the parameters θ : $P(\mathbf{t}, \mathbf{z}|\theta)$. Which can be written as a conditional distribution:

$$P(\mathbf{t}, \mathbf{z}|\theta) = P(\mathbf{t}|\mathbf{z}, \theta)P(\mathbf{z}|\theta)$$

Since we are not interested in the probability of \mathbf{z} we can reduce this to: $\mathcal{L}(\theta|\mathbf{t}, \mathbf{z}) = P(\mathbf{t}|\mathbf{z}, \theta)$. Which can be written as $P(\mathbf{t}|\mathbf{z})$ for fixed θ . Since each t_c is dependent on the full \mathbf{z} , and only 1 class can be activated in the \mathbf{t} we can write

$$P(\mathbf{t}|\mathbf{z}) = \prod_{i=c}^C P(t_c|\mathbf{z})^{t_c} = \prod_{c=1}^C \varsigma(\mathbf{z})_c^{t_c} = \prod_{c=1}^C y_c^{t_c}$$

Cross-entropy loss function for the softmax function

$$P(\mathbf{t}|\mathbf{z}) = \prod_{i=c}^C P(t_c|\mathbf{z})^{t_c} = \prod_{c=1}^C \varsigma(\mathbf{z})_c^{t_c} = \prod_{c=1}^C y_c^{t_c}$$

As was noted during the derivation of the loss function of the logistic function, maximizing this likelihood can also be done by minimizing the negative log-likelihood:

$$-\log \mathcal{L}(\theta|\mathbf{t}, \mathbf{z}) = \xi(\mathbf{t}, \mathbf{z}) = -\log \prod_{c=1}^C y_c^{t_c} = \sum_{c=1}^C t_c \cdot \log(y_c)$$

Cross-entropy loss function for the softmax function

$$-\log \mathcal{L}(\theta|\mathbf{t}, \mathbf{z}) = \xi(\mathbf{t}, \mathbf{z}) = -\log \prod_{c=1}^C y_c^{t_c} = \sum_{c=1}^C t_c \cdot \log(y_c)$$

The cross-entropy error function over a batch of multiple samples of size n can be calculated as:

$$\xi(T, Y) = \sum_{i=1}^n \xi(\mathbf{t}_i, \mathbf{y}_i) = -\sum_{i=1}^n \sum_{c=1}^C t_{ic} \cdot \log(y_{ic})$$

Where t_{ic} is 1 if and only if sample i belongs to class c , and y_{ic} is the output probability that sample i belongs to class c .

Derivative of the cross-entropy loss function for the softmax function

The derivative $\partial \xi / \partial z_i$ of the loss function with respect to the softmax input z_i can be calculated as:

$$\begin{aligned}\frac{\partial \xi}{\partial z_i} &= - \sum_{j=1}^C \frac{\partial t_j \log(y_j)}{\partial z_i} = - \sum_{j=1}^C t_j \frac{\partial \log(y_j)}{\partial z_i} = - \sum_{j=1}^C t_j \frac{1}{y_j} \frac{\partial y_j}{\partial z_i} \\&= - \frac{t_i}{y_i} \frac{\partial y_i}{\partial z_i} - \sum_{j \neq i}^C \frac{t_j}{y_j} \frac{\partial y_j}{\partial z_i} = - \frac{t_i}{y_i} y_i (1 - y_i) - \sum_{j \neq i}^C \frac{t_j}{y_j} (-y_j y_i) \\&= -t_i + t_i y_i + \sum_{j \neq i}^C t_j y_i = -t_i + \sum_{j=1}^C t_j y_i = -t_i + y_i \sum_{j=1}^C t_j \\&= y_i - t_i\end{aligned}$$

Derivative of the cross-entropy loss function for the softmax function

$$\frac{\partial \xi}{\partial z_i} = y_i - t_i$$

$$\text{if } i = j : \frac{\partial y_i}{\partial z_i} = \frac{\partial \frac{e^{z_i}}{\Sigma_C}}{\partial z_i} = \frac{e^{z_i} \Sigma_C - e^{z_i} e^{z_i}}{\Sigma_C^2} = \frac{e^{z_i}}{\Sigma_C} \frac{\Sigma_C - e^{z_i}}{\Sigma_C} = \frac{e^{z_i}}{\Sigma_C} \left(1 - \frac{e^{z_i}}{\Sigma_C}\right) = y_i(1 - y_i)$$

$$\text{if } i \neq j : \frac{\partial y_i}{\partial z_j} = \frac{\partial \frac{e^{z_i}}{\Sigma_C}}{\partial z_j} = \frac{0 - e^{z_i} e^{z_j}}{\Sigma_C^2} = -\frac{e^{z_i}}{\Sigma_C} \frac{e^{z_j}}{\Sigma_C} = -y_i y_j$$

Derivative of the cross-entropy loss function for the softmax function

$$\frac{\partial \xi}{\partial z_i} = y_i - t_i$$

$$\text{if } i = j : \frac{\partial y_i}{\partial z_i} = \frac{\partial \frac{e^{z_i}}{\Sigma_C}}{\partial z_i} = \frac{e^{z_i} \Sigma_C - e^{z_i} e^{z_i}}{\Sigma_C^2} = \frac{e^{z_i}}{\Sigma_C} \frac{\Sigma_C - e^{z_i}}{\Sigma_C} = \frac{e^{z_i}}{\Sigma_C} \left(1 - \frac{e^{z_i}}{\Sigma_C}\right) = y_i(1 - y_i)$$

$$\text{if } i \neq j : \frac{\partial y_i}{\partial z_j} = \frac{\partial \frac{e^{z_i}}{\Sigma_C}}{\partial z_j} = \frac{0 - e^{z_i} e^{z_j}}{\Sigma_C^2} = -\frac{e^{z_i}}{\Sigma_C} \frac{e^{z_j}}{\Sigma_C} = -y_i y_j$$

$$\frac{\partial z_i}{\partial w_j} = ?$$

Gradient Descent?

Example of Softmax and classification

- <https://medium.com/@awjuliani/simple-softmax-in-python-tutorial-d6b4c4ed5c16>
- <https://www.kaggle.com/saksham219/softmax-regression-for-iris-classification>
- https://scikit-learn.org/stable/auto_examples/linear_model/plot_iris_logistic.html